@prefix cr: <http://mlcommons.org/croissant/> .
@prefix owl: <http://www.w3.org/2002/07/owl#> .
@prefix rdfs: <http://www.w3.org/2000/01/rdf-schema#> .
@prefix schema: <https://schema.org/> .
@prefix skos: <http://www.w3.org/2004/02/skos/core#> .

cr:field a owl:ObjectProperty ;
    rdfs:domain cr:RecordSet ;
    rdfs:range cr:Field ;
    skos:definition "Ein Datenelement, das in den Eintr채gen eines RecordSets erscheint (z.B. eine Spalte einer Tabelle)"@de,
        "A data element that appears in the records of the RecordSet (e.g., one column of a table)."@en ;
    skos:editorialNote "changed by m4i: added skos:prefLabel and skos:definition, added german labels, removed schema:rangeIncludes and schema:domainIncludes properties"@en ;
    skos:prefLabel "hat Feld"@de,
        "field"@en .

cr:Field a owl:Class ;
    rdfs:subClassOf schema:Intangible ;
    skos:definition "Ein Bestandteil der Struktur eines RecordSets wie z.B. eine Spalte einer Tabelle"@de,
        "A component of the structure of a RecordSet, such as a column of a table."@en ;
    skos:editorialNote "changed by m4i: added german labels, added skos:prefLabel and skos:definition"@en ;
    skos:prefLabel "Feld"@de,
        "Field"@en .

cr:RecordSet a owl:Class ;
    rdfs:subClassOf schema:Intangible ;
    skos:definition "Eine Beschreibung einer Menge strukturierter Eintr채ge von einer oder mehrerer Datenquellen mit ihrer Struktur, ausgedr체ckt durch eine Menge von Feldern"@de,
        "A description of a set of structured records from one or more data sources and their structure, expressed as a set of fields."@en ;
    skos:editorialNote "changed by m4i: added german labels, added skos:prefLabel and skos:definition, harmonized spelling to OBO naming conventions (lower case, space separated)"@en ;
    skos:prefLabel "Menge von Eintr채gen"@de,
        "record set"@en .

schema:Intangible a owl:Class ;
    skos:definition "A utility class that serves as the umbrella for a number of 'intangible' things such as quantities, structured values, etc."@en ;
    skos:editorialNote "changed by m4i: added skos:prefLabel, added german label, harmonized spelling to OBO naming conventions (lower case, space separated)"@en ;
    skos:prefLabel "Ungreifbares"@de,
        "intangible"@en .

