@prefix foaf: <http://xmlns.com/foaf/0.1/> .
@prefix m4i: <http://w3id.org/nfdi4ing/metadata4ing#> .
@prefix owl: <http://www.w3.org/2002/07/owl#> .
@prefix prov: <http://www.w3.org/ns/prov#> .
@prefix rdf: <http://www.w3.org/1999/02/22-rdf-syntax-ns#> .
@prefix rdfs: <http://www.w3.org/2000/01/rdf-schema#> .
@prefix skos: <http://www.w3.org/2004/02/skos/core#> .
@prefix xsd: <http://www.w3.org/2001/XMLSchema#> .

m4i:orcidId a owl:DatatypeProperty ;
    rdfs:domain prov:Person ;
    rdfs:range [ a rdfs:Datatype ;
            owl:onDatatype xsd:string ;
            owl:withRestrictions ( [ xsd:pattern "https://orcid.org/[0-9][0-9][0-9][0-9]-[0-9][0-9][0-9][0-9]-[0-9][0-9][0-9][0-9]-[0-9][0-9][0-9][0-9X]" ] ) ] ;
    rdfs:subPropertyOf m4i:identifier ;
    skos:definition "Open Researcher and Contributor ID: ein persistenter Identifikator, der eine in der Forschung tätige Person eindeutig identifiziert."@de,
        "Open Researcher and Contributor ID: an identifier, that allows unique identification of a person, usually active in research."@en ;
    skos:prefLabel "hat ORCID ID"@de,
        "has ORCID ID"@en .

foaf:Person a owl:Class ;
    rdfs:comment "DEPRECATED A person.",
        "Replace foaf:Person by prov:Person" ;
    rdfs:seeAlso prov:Person ;
    rdfs:subClassOf foaf:Agent ;
    owl:deprecated true .

m4i:identifier a owl:DatatypeProperty ;
    rdfs:domain owl:Thing ;
    rdfs:range xsd:string ;
    skos:altLabel "besitzt eindeutigen Identifikator"@de,
        "wird durch Identifikator repräsentiert"@de,
        "has unique identifier"@en,
        "is represented through identifier"@en ;
    skos:definition "A systematically built alphanumeric string that identifies a unique object (e.g. a person, a publication, an organisation, a research activity, a sample, etc.) or a unique class of objects."@en ;
    skos:prefLabel "hat Identifikator"@de,
        "has identifier"@en .

foaf:Agent a owl:Class ;
    rdfs:comment "DEPRECATED An agent (eg. person, group, software or physical artifact).",
        "exchanged foaf:Agent by prov:Agent to fulfill range definition of prov:agent property" ;
    rdfs:seeAlso prov:Agent ;
    owl:deprecated true .

